Backing up the type system

while-program-infoflow/NTNITypeSystem.dfy
@@ -10,28 +10,48 @@ module NontransitiveFlow{
     // The security labels
     type Label(==)
     const labels: set<Label>
-    // The reflexive flow relation on Labels
+    // The reflexive flow relation on Labels, which is a global policy
     const flow: set<(Label, Label)>
-    lemma {: axiom} ReflexiveFlow(l: Label)
-    requires l in labels 
-    ensures (l, l) in flow
+    // lemma {: axiom} ReflexiveFlow(l: Label)
+    // requires l in labels 
+    // ensures (l, l) in flow
+    // An initial labelling on variables
+    // Intuitively, an "unimportant" variable may be labelled by \top 
+    // which may influence any other labels and may accept information flow from any other labels
+    const coarse_label: map<Variable, Label>
+    predicate policyTypeOK(){
+        && coarse_label.Keys == variables
+        && (forall l :: l in labels ==> (l, l) in flow)
+        && forall x :: x in variables ==> coarse_label[x] in labels
+    }
 
     // The set of labels that can interfere with a label
-    method CanFlow(l: Label) returns (incoming: set<Label>)
+    // method CanFlow(l: Label) returns (incoming: set<Label>)
+    // requires l in labels
+    // ensures forall l':: l' in labels && (l',l) in flow ==> l' in incoming
+    // ensures forall l':: l' in incoming ==> (l', l) in flow
+    // ensures incoming <= labels
+    // {
+    //     incoming := (set l' | l' in labels && (l', l) in flow :: l');
+    //     // assert forall l':: l' in labels && (l',l) in flow ==> l' in incoming;
+    //     // assert forall l':: l' in incoming ==> (l', l) in flow;
+    // }
+    function CanFlow(l: Label): set<Label>
     requires l in labels
-    ensures forall l':: l' in labels && (l',l) in flow ==> l' in incoming
-    ensures forall l':: l' in incoming ==> (l', l) in flow
+    ensures forall l':: l' in labels && (l',l) in flow ==> l' in CanFlow(l)
+    ensures forall l':: l' in CanFlow(l) ==> (l', l) in flow
+    ensures CanFlow(l) <= labels
     {
-        incoming := (set l' | l' in labels && (l', l) in flow :: l');
-        // assert forall l':: l' in labels && (l',l) in flow ==> l' in incoming;
-        // assert forall l':: l' in incoming ==> (l', l) in flow;
+        (set l' | l' in labels && (l', l) in flow :: l')
     }
+
     // Testing for all labels l, l is in the set of labels in CanFlow(l)
     method TestSelfFlow(l: Label)
     requires l in labels
+    requires policyTypeOK()
     {
         var lset := CanFlow(l);
-        ReflexiveFlow(l);
+        // ReflexiveFlow(l);
         assert l in lset;
     }
 
@@ -59,7 +79,7 @@ module NontransitiveFlow{
     }
     // The following defines a type system for the while programming language
     // We start with the expression types
-    // This function never produces Invalid
+    //// In principle, this function should never produce Invalid
     function HasExprType(ctx: Context, e: Expr): PhraseType
     requires VariablesInExpr(e) <= ctx.Keys
     decreases e
@@ -73,6 +93,30 @@ module NontransitiveFlow{
                 var t1, t2 := HasExprType(ctx, e1), HasExprType(ctx, e2); 
                 if t1 == Invalid || t2 == Invalid then Invalid 
                 else ExprType(Join(GetBaseType(t1), GetBaseType(t2)))
+        }
+    }
+    // The type checking process for a command/statement
+    // If type checking fails the return type will be Invalid
+    function HasCmdType(ctx: Context, pc: set<Label>, c:Cmd): PhraseType
+    requires policyTypeOK()
+    requires VariablesInCmd(c) <= ctx.Keys && pc <= labels
+    requires VariablesInCmd(c) <= variables
+    requires forall x :: x in ctx.Keys ==> ctx[x] <= labels
+    {
+        match c {
+            case Skip => CmdType({})
+            case Assn(x, e) =>  
+                // t1 is the policy label of x; t2 represents information from RHS of assn
+                var t1, t2 := coarse_label[x], HasExprType(ctx, e); 
+                if t2 == Invalid then Invalid
+                else 
+                    // get the set of labels allowed to influence label(x)
+                    var flowsFrom := CanFlow(t1); 
+                    if (GetBaseType(t2) + pc) <= ctx[x] && (GetBaseType(t2) + pc) <= flowsFrom
+                    then CmdType({t1}) else Invalid
+            case If(e, c1, c2) => CmdType({})
+            case While(e, c1) => CmdType({})
+            case Seq(c1, c2) => CmdType({})
         }
     }
 }
